Rename `Kind` to `CapKind`

Semantic/CaplessK/Syntax/Classifier/CapKind.lean
@@ -3,7 +3,7 @@ import Semantic.CaplessK.Syntax.Classifier.Core
 namespace CaplessK
 
 -- **
--- Kinds
+-- CapKinds
 -- **
 
 /-- A subtree of a single root and an exclusion list.
@@ -15,29 +15,29 @@ structure Subtree : Type where
 deriving DecidableEq
 
 /-- A classifier filter : a list of filtered subtree. -/
-def Kind : Type := List Subtree
+def CapKind : Type := List Subtree
 
 @[simp]
-instance : HAppend Kind Kind Kind where
+instance : HAppend CapKind CapKind CapKind where
   hAppend xs ys := List.append xs ys
 
 /-- A single node. -/
 @[simp]
-def Kind.node (c : Classifier) (excls : List Classifier) : Kind := [Subtree.mk c excls]
+def CapKind.node (c : Classifier) (excls : List Classifier) : CapKind := [Subtree.mk c excls]
 
 /-- Shorthand notation for a subtree without exclusions -/
 @[simp]
-def Kind.classifier (c : Classifier) := Kind.node c []
+def CapKind.classifier (c : Classifier) := CapKind.node c []
 
 /-- The empty kind.
     Note that non-empty kinds can still represent an empty set of nodes.
     See `IsEmpty`. -/
 @[simp]
-def Kind.empty : Kind := []
+def CapKind.empty : CapKind := []
 
-/-- The "top" kind. This is a Kind that includes all nodes in the classifier tree. -/
+/-- The "top" kind. This is a CapKind that includes all nodes in the classifier tree. -/
 @[simp]
-def Kind.top := node .top []
+def CapKind.top := node .top []
 
 /-- Helper relation: does `xs` contain a superclass of `c`? -/
 inductive ContainsSupOf : List Classifier -> Classifier -> Prop where
@@ -96,12 +96,12 @@ theorem ContainsSupOf.of_append
       | inl h => exact .inl (.there h)
       | inr h => exact .inr h
 
-/-- Is a Kind empty? -/
-inductive Kind.IsEmpty : Kind -> Prop where
+/-- Is a CapKind empty? -/
+inductive CapKind.IsEmpty : CapKind -> Prop where
   | empty : IsEmpty []
   | absurd : ContainsSupOf exs r -> IsEmpty xs -> IsEmpty (Subtree.mk r exs :: xs)
 
-instance Kind.IsEmpty.decidable : Decidable (IsEmpty K) := by
+instance CapKind.IsEmpty.decidable : Decidable (IsEmpty K) := by
   cases K
   case nil => apply isTrue .empty
   case cons x xs =>
@@ -112,13 +112,13 @@ instance Kind.IsEmpty.decidable : Decidable (IsEmpty K) := by
     rename_i h1 h2
     apply isTrue (.absurd h1 h2)
 
-theorem Kind.IsEmpty.node (hsc : ContainsSupOf exs r) : IsEmpty [.mk r exs] := absurd hsc .empty
+theorem CapKind.IsEmpty.node (hsc : ContainsSupOf exs r) : IsEmpty [.mk r exs] := absurd hsc .empty
 
 /-- If a `node` is empty, it is absurd. -/
-theorem Kind.IsEmpty.is_absurd (he : IsEmpty (.node r exs)) : ContainsSupOf exs r := by
+theorem CapKind.IsEmpty.is_absurd (he : IsEmpty (.node r exs)) : ContainsSupOf exs r := by
   cases he; assumption
 
-theorem Kind.IsEmpty.append (he1 : IsEmpty R1) (he2 : IsEmpty R2) : IsEmpty (R1 ++ R2) := by
+theorem CapKind.IsEmpty.append (he1 : IsEmpty R1) (he2 : IsEmpty R2) : IsEmpty (R1 ++ R2) := by
   induction R1 generalizing R2
   case nil => simp_all
   case cons x xs ih =>
@@ -126,7 +126,7 @@ theorem Kind.IsEmpty.append (he1 : IsEmpty R1) (he2 : IsEmpty R2) : IsEmpty (R1 
     cases he1
     apply! absurd _ (ih _ _)
 
-theorem Kind.IsEmpty.append_inv (he : IsEmpty (R1 ++ R2)) : IsEmpty R1 ∧ IsEmpty R2 := by
+theorem CapKind.IsEmpty.append_inv (he : IsEmpty (R1 ++ R2)) : IsEmpty R1 ∧ IsEmpty R2 := by
   induction R1 generalizing R2
   case nil => simp_all; apply empty
   case cons x xs ih =>
