Semantic/CaplessK/Syntax/Classifier/Disjoint.lean
@@ -1,17 +1,17 @@
-import Semantic.CaplessK.Syntax.Classifier.Kind
+import Semantic.CaplessK.Syntax.Classifier.CapKind
 import Semantic.CaplessK.Syntax.Classifier.Intersection
 import Semantic.CaplessK.Syntax.Classifier.Semantics
 
 namespace CaplessK
 
 /-- Two subtrees are disjoint if they do not share any common nodes. -/
-inductive Kind.Disjoint : Kind -> Kind -> Prop where
+inductive CapKind.Disjoint : CapKind -> CapKind -> Prop where
   | intersect : Intersect K L R -> R.IsEmpty -> Disjoint K L
 
-/-- Decides whether two Kinds are disjoint. -/
-def Kind.disjoint (a b : Kind) := (IsEmpty.decidable (K:=a.intersect b)).decide
+/-- Decides whether two CapKinds are disjoint. -/
+def CapKind.disjoint (a b : CapKind) := (IsEmpty.decidable (K:=a.intersect b)).decide
 
-theorem Kind.Disjoint.empty_intersect : IsEmpty (K.intersect L) ↔ Disjoint K L := by
+theorem CapKind.Disjoint.empty_intersect : IsEmpty (K.intersect L) ↔ Disjoint K L := by
   apply Iff.intro <;> intro h
   · apply intersect (Intersect.lawful _ _) h
   · cases h
@@ -24,11 +24,11 @@ theorem Kind.Disjoint.empty_intersect : IsEmpty (K.intersect L) ↔ Disjoint K L
     apply! h1.contains
 
 /-- Proves that `disjoint` follows derivation. -/
-theorem Kind.disjoint.lawful : Disjoint K L ↔ disjoint K L := by
+theorem CapKind.disjoint.lawful : Disjoint K L ↔ disjoint K L := by
   rw [disjoint, decide_eq_true_iff]
   exact Disjoint.empty_intersect.symm
 
-theorem Kind.Disjoint.symm (hs : Disjoint K L) : Disjoint L K := by
+theorem CapKind.Disjoint.symm (hs : Disjoint K L) : Disjoint L K := by
   cases hs
   rename_i h1 h2
   have h := Intersect.lawful L K
@@ -39,11 +39,11 @@ theorem Kind.Disjoint.symm (hs : Disjoint K L) : Disjoint L K := by
   have ⟨_, _⟩ := h.contains_inv hc
   apply! h1.contains
 
-theorem Kind.disjoint.symm (hs : disjoint K L) : disjoint L K := by
+theorem CapKind.disjoint.symm (hs : disjoint K L) : disjoint L K := by
   rw [← lawful] at *
   apply! Disjoint.symm
 
-theorem Kind.Disjoint.union_l
+theorem CapKind.Disjoint.union_l
     (hd1 : Disjoint K1 L) (hd2 : Disjoint K2 L) : Disjoint (K1 ++ K2) L := by
   rw [← empty_intersect, ← SEmpty.is_empty] at *
   intro c hc
@@ -55,7 +55,7 @@ theorem Kind.Disjoint.union_l
   · apply hd1 c; apply! h1.contains
   · apply hd2 c; apply! h2.contains
 
-theorem Kind.Disjoint.is_empty_l (he : IsEmpty K) : Disjoint K L := by
+theorem CapKind.Disjoint.is_empty_l (he : IsEmpty K) : Disjoint K L := by
   rw [← empty_intersect, ← SEmpty.is_empty] at *
   intro c hc
   apply he c
@@ -63,7 +63,7 @@ theorem Kind.Disjoint.is_empty_l (he : IsEmpty K) : Disjoint K L := by
   have ⟨_, _⟩ := h.contains_inv hc
   assumption
 
-theorem Kind.Disjoint.is_empty_r (he : IsEmpty L) : Disjoint K L := by
+theorem CapKind.Disjoint.is_empty_r (he : IsEmpty L) : Disjoint K L := by
   rw [← empty_intersect, ← SEmpty.is_empty] at *
   intro c hc
   apply he c
