Semantic/CaplessK/Syntax/Classifier/Intersection.lean
@@ -1,16 +1,16 @@
 import Semantic.CaplessK.Syntax.Classifier.Core
-import Semantic.CaplessK.Syntax.Classifier.Kind
+import Semantic.CaplessK.Syntax.Classifier.CapKind
 
 namespace CaplessK
 
 /-- The intersection of two subtrees. -/
-inductive Subtree.Intersect : Subtree -> Subtree -> Kind -> Prop where
+inductive Subtree.Intersect : Subtree -> Subtree -> CapKind -> Prop where
   | subtree_l : r1.Subclass r2 -> Intersect (mk r1 ex1) (mk r2 ex2) [mk r1 (ex1 ++ ex2)]
   | subtree_r : r2.Subclass r1 -> Intersect (mk r1 ex1) (mk r2 ex2) [mk r2 (ex1 ++ ex2)]
   | disjoint : r1.Disjoint r2 -> Intersect (mk r1 ex1) (mk r2 ex2) []
 
 /-- Intersection of two kinds. -/
-inductive Kind.Intersect : Kind -> Kind -> Kind -> Prop where
+inductive CapKind.Intersect : CapKind -> CapKind -> CapKind -> Prop where
   | empty_l : Intersect [] K []
   | empty_r : Intersect K [] []
   | append_l : Intersect [x] K R1 -> Intersect xs K R2 -> Intersect (x::xs) K (R1 ++ R2)
@@ -18,7 +18,7 @@ inductive Kind.Intersect : Kind -> Kind -> Kind -> Prop where
   | singleton : x.Intersect y R -> Intersect [x] [y] R
 
 @[simp]
-def Subtree.intersect (s : Subtree) (t : Subtree) : Kind :=
+def Subtree.intersect (s : Subtree) (t : Subtree) : CapKind :=
   if s.root.subclass t.root then .node s.root (s.excls ++ t.excls)
   else if t.root.subclass s.root then .node t.root (s.excls ++ t.excls)
   else .empty
@@ -41,21 +41,21 @@ theorem Subtree.Intersect.lawful : Intersect s t (s.intersect t) := by
         · apply! disjoint
 
 @[simp]
-def Kind.intersect (k : Kind) (l : Kind) : Kind :=
+def CapKind.intersect (k : CapKind) (l : CapKind) : CapKind :=
   List.flatMap (fun x => List.flatMap (fun y => x.intersect y) l) k
 
-theorem Kind.intersect.cons_l : intersect (x :: xs) K = intersect [x] K ++ intersect xs K := by simp
+theorem CapKind.intersect.cons_l : intersect (x :: xs) K = intersect [x] K ++ intersect xs K := by simp
 
-theorem Kind.intersect.append_l :
+theorem CapKind.intersect.append_l :
     intersect (xs1 ++ xs2) K = intersect xs1 K ++ intersect xs2 K := by simp
 
-theorem Kind.intersect.cons_r :
+theorem CapKind.intersect.cons_r :
     intersect [x] (y :: ys) = intersect [x] [y] ++ intersect [x] ys := by simp
 
-theorem Kind.intersect.append_r :
+theorem CapKind.intersect.append_r :
     intersect [x] (ys1 ++ ys2) = intersect [x] ys1 ++ intersect [x] ys2 := by simp
 
-theorem Kind.Intersect.lawful' : Intersect [x] L (.intersect [x] L) := by
+theorem CapKind.Intersect.lawful' : Intersect [x] L (.intersect [x] L) := by
   induction L
   case nil => simp; apply empty_r
   case cons y ys ih =>
@@ -64,7 +64,7 @@ theorem Kind.Intersect.lawful' : Intersect [x] L (.intersect [x] L) := by
     · apply singleton .lawful
     · simp at ih; apply ih
 
-theorem Kind.Intersect.lawful (K L : Kind) : Intersect K L (K.intersect L) := by
+theorem CapKind.Intersect.lawful (K L : CapKind) : Intersect K L (K.intersect L) := by
   induction K generalizing L
   case nil => simp; apply empty_l
   case cons x xs ih =>
@@ -72,7 +72,7 @@ theorem Kind.Intersect.lawful (K L : Kind) : Intersect K L (K.intersect L) := by
     have h := lawful' (x:=x) (L:=L)
     simp_all
 
-theorem Kind.intersect.top_r {K : Kind} : K.intersect .top = K := by
+theorem CapKind.intersect.top_r {K : CapKind} : K.intersect .top = K := by
   induction K
   case nil => simp
   case cons x xs ih =>
@@ -81,7 +81,7 @@ theorem Kind.intersect.top_r {K : Kind} : K.intersect .top = K := by
     rw [cons_l, ih]
     simp [h]
 
-theorem Kind.intersect.top_l {K : Kind} : Kind.top.intersect K = K := by
+theorem CapKind.intersect.top_l {K : CapKind} : CapKind.top.intersect K = K := by
   induction K
   case nil => simp
   case cons y ys ih =>
@@ -110,7 +110,7 @@ theorem Classifier.StrictSub.not_superclass (hss : StrictSub a b) : (b.subclass 
   intro h
   apply hss.antisymm h
 
-theorem Kind.intersect.assoc'' :
+theorem CapKind.intersect.assoc'' :
     (intersect [x] [y]).intersect [z] = intersect [x] (intersect [y] [z]) := by
   cases Classifier.subclass_or_disjoint x.root y.root <;> rename_i h1
   · have h1' := Classifier.subclass_is_Subclass.mp h1
@@ -159,7 +159,7 @@ theorem Kind.intersect.assoc'' :
             Classifier.disjoint_is_Disjoint.mp h2
           simp_all
 
-theorem Kind.intersect.assoc' {B C : Kind} :
+theorem CapKind.intersect.assoc' {B C : CapKind} :
     (intersect [x] B).intersect C = intersect [x] (B.intersect C) := by
   induction B generalizing C
   case nil => simp
@@ -178,7 +178,7 @@ theorem Kind.intersect.assoc' {B C : Kind} :
           · subst_vars; simp
       rw [cons_r (ys:=zs), append_r, h, assoc'', ih2]
 
-theorem Kind.intersect.assoc {A B C : Kind} :
+theorem CapKind.intersect.assoc {A B C : CapKind} :
     (A.intersect B).intersect C = A.intersect (B.intersect C) := by
   induction A generalizing B C
   case nil => simp
