Semantic/CaplessK/Syntax/Classifier.lean
@@ -1,5 +1,5 @@
 import Semantic.CaplessK.Syntax.Classifier.Core
-import Semantic.CaplessK.Syntax.Classifier.Kind
+import Semantic.CaplessK.Syntax.Classifier.CapKind
 import Semantic.CaplessK.Syntax.Classifier.Subtract
 import Semantic.CaplessK.Syntax.Classifier.Intersection
 import Semantic.CaplessK.Syntax.Classifier.Semantics
