Semantic/CaplessK/Syntax/Classifier/Basic.lean
@@ -5,7 +5,7 @@ import Semantic.CaplessK.Syntax.Classifier.Disjoint
 
 namespace CaplessK
 
-theorem Kind.Intersect.with_subkind
+theorem CapKind.Intersect.with_subkind
     (hs : K1.Subkind K2)
     : (intersect L K1).Subkind (intersect L K2) := by
   rw [Subkind.semantics] at *
@@ -13,7 +13,7 @@ theorem Kind.Intersect.with_subkind
   have h2 := Intersect.lawful L K2
   apply! Intersect.with_ssubkind_l
 
-theorem Kind.Intersect.with_subkind_r
+theorem CapKind.Intersect.with_subkind_r
     (hs : K1.Subkind K2)
     : (intersect K1 L).Subkind (intersect K2 L) := by
   rw [Subkind.semantics] at *
@@ -21,19 +21,19 @@ theorem Kind.Intersect.with_subkind_r
   have h2 := Intersect.lawful K2 L
   apply! Intersect.with_ssubkind_r
 
-theorem Kind.Intersect.subkind_l
+theorem CapKind.Intersect.subkind_l
     : (intersect K L).Subkind K := by
   rw [Subkind.semantics]
   have h := Intersect.lawful K L
   apply h.is_ssubkind_l
 
-theorem Kind.Intersect.subkind_r
+theorem CapKind.Intersect.subkind_r
     : (intersect K L).Subkind L := by
   rw [Subkind.semantics]
   have h := Intersect.lawful K L
   apply h.is_ssubkind_r
 
-theorem Kind.Subkind.reorder_union_4 : Subkind ((A ++ B) ++ (C ++ D)) ((A ++ C) ++ (B ++ D)) := by
+theorem CapKind.Subkind.reorder_union_4 : Subkind ((A ++ B) ++ (C ++ D)) ((A ++ C) ++ (B ++ D)) := by
   apply union_l
   · apply union_l
     · apply trans .union_rl .union_rl
@@ -42,7 +42,7 @@ theorem Kind.Subkind.reorder_union_4 : Subkind ((A ++ B) ++ (C ++ D)) ((A ++ C) 
     · apply trans .union_rr .union_rl
     · apply trans .union_rr .union_rr
 
-theorem Kind.Intersect.union_r_subkind :
+theorem CapKind.Intersect.union_r_subkind :
     Subkind (.intersect K (L1 ++ L2)) ((K.intersect L1) ++ (K.intersect L2)) := by
   rw [Subkind.semantics]
   intro c hc
@@ -54,7 +54,7 @@ theorem Kind.Intersect.union_r_subkind :
   · apply Contains.append_r; apply hi1.contains h1 h2
   · apply Contains.append_l; apply hi2.contains h1 h2
 
-theorem Kind.Intersect.union_r_superkind :
+theorem CapKind.Intersect.union_r_superkind :
     Subkind ((K.intersect L1) ++ (K.intersect L2)) (.intersect K (L1 ++ L2)) := by
   rw [Subkind.semantics]
   intro c hc
@@ -67,13 +67,13 @@ theorem Kind.Intersect.union_r_superkind :
   · have ⟨hc1, hc2⟩ := hi2.contains_inv hc
     apply contains hi hc1 (.append_l hc2)
 
-theorem Kind.Intersect.subkind_self : Subkind A (.intersect A A) := by
+theorem CapKind.Intersect.subkind_self : Subkind A (.intersect A A) := by
   rw [Subkind.semantics]
   intro c hc
   have hi := Intersect.lawful A A
   apply! hi.contains
 
-theorem Kind.Intersect.is_empty_repeat
+theorem CapKind.Intersect.is_empty_repeat
     (he : IsEmpty (.intersect A (.intersect B A))) : IsEmpty (.intersect B A) := by
   rw [← SEmpty.is_empty] at *
   intro c hc
@@ -83,7 +83,7 @@ theorem Kind.Intersect.is_empty_repeat
   have ⟨_, _⟩ := hi.contains_inv hc
   apply! hi'.contains
 
-theorem Kind.Intersect.subkind_symm : Subkind (.intersect A B) (.intersect B A) := by
+theorem CapKind.Intersect.subkind_symm : Subkind (.intersect A B) (.intersect B A) := by
   rw [Subkind.semantics]
   intro c hc
   have ha := Intersect.lawful A B
@@ -93,7 +93,7 @@ theorem Kind.Intersect.subkind_symm : Subkind (.intersect A B) (.intersect B A) 
 
 -- Disjointness and Subkinding
 
-theorem Kind.Disjoint.refine_subkind_l
+theorem CapKind.Disjoint.refine_subkind_l
     (hd : Disjoint K2 L)
     (hs : K1.Subkind K2)
     : Disjoint K1 L := by
@@ -106,28 +106,28 @@ theorem Kind.Disjoint.refine_subkind_l
   have hc2 := hs c hc1
   apply! h2.contains
 
-theorem Kind.disjoint.refine_subkind_l
+theorem CapKind.disjoint.refine_subkind_l
     (hd : disjoint K2 L) (hs : K1.Subkind K2) : disjoint K1 L := by
   rw [← disjoint.lawful] at *; apply! Disjoint.refine_subkind_l
 
-theorem Kind.Disjoint.refine_subkind_r
+theorem CapKind.Disjoint.refine_subkind_r
     (hd : Disjoint L K2)
     (hs : K1.Subkind K2)
     : Disjoint L K1 := by
   apply symm; apply! hd.symm.refine_subkind_l
 
-theorem Kind.disjoint.refine_subkind_r
+theorem CapKind.disjoint.refine_subkind_r
     (hd : disjoint L K2) (hs : K1.Subkind K2) : disjoint L K1 := by
   rw [← disjoint.lawful] at *; apply! Disjoint.refine_subkind_r
 
-theorem Kind.Disjoint.and_subkind (hd : Disjoint K L) (hs : K.Subkind L) : K.IsEmpty := by
+theorem CapKind.Disjoint.and_subkind (hd : Disjoint K L) (hs : K.Subkind L) : K.IsEmpty := by
   rw [← Disjoint.empty_intersect, Subkind.semantics, ← SEmpty.is_empty] at *
   intro c hc
   apply hd c
   have hi := Intersect.lawful K L
   apply hi.contains hc (hs c hc)
 
-theorem Kind.Disjoint.with_self (hd : Disjoint K K) : K.IsEmpty := by
+theorem CapKind.Disjoint.with_self (hd : Disjoint K K) : K.IsEmpty := by
   apply hd.and_subkind .rfl
 
 end CaplessK
